

Sigma Notation {data-navmenu="Section 5"}
==================================

Column {.tabset}
-----------------------------


### Cartesian Product

A ***Cartesian product*** is a mathematical operation which returns a set (or product set) from multiple sets. 
 
That is, for sets A and B, the Cartesian product $A \times B$ is the set of all ordered pairs $(a, b)$ where $a \in A$ and $b \in B$.


### Power Series



* In mathematics, a power series (in one variable) is an infinite series of the form
\[f(x) = \sum_{n=0}^\infty a_n \left( x-c \right)^n = a_0 + a_1 (x-c)^1 + a_2 (x-c)^2 + a_3 (x-c)^3 + \cdots\]
where an represents the coefficient of the nth term, c is a constant, and x varies around c (for this reason one sometimes speaks of the series as being centered at c).
* This series usually arises as the Taylor series of some known function.

* In many situations c is equal to zero, for instance when considering a Maclaurin series. 
* In such cases, the power series takes the simpler form

\[f(x) = \sum_{n=0}^\infty a_n x^n = a_0 + a_1 x + a_2 x^2 + a_3 x^3 + \cdots.\]



### Sigma Notation

<h4> Sigma Notation</h4>
Instead of writing out a long sum for every term in a series, the greek letter Sigma is used to denote such sums. For a sum over a range or terms $a_p$ to $a_q$, with $p<q$ let
$$
  \sum_{k=p}^{q}a_k = a_p+a_{p+1}+a_{p+2}+a_{p+3}+\cdots+a_{q-1}+a_q
$$
* The sum is over the variable $k$ which ranges from the lower bound $p$, increasing in steps of $1$, until it reaches the upper bound $q$. 
* The Sigma denotes that all the terms are to be added together. With this, the general term $s_n$ in the sequence is written
\begin{multicols}{2}
$\qquad \qquad s_n=\displaystyle \sum_{k=0}^n a_k$


or $\ s_n=\displaystyle \sum_{k=1}^n a_k\quad $ if $a_0$ is not defined.
\end{multicols}
\pagebreak

* \textbf{Example:} Sum of first $n$ integers
$$
  s_n=\sum_{k=0}^n k = 0 + 1 + 2 + 3 + \cdots + (n-1) + n 
$$
\[
\begin{array}{c|c|c|c|c|c|c|c|c|c|c|c}
$n$ & $0$ & $1$ & $2$ & $3$ & $4$ & $5$ & $6$ & $7$ & $8$ & $9$ & $10$  \hline
$a_n$ & $0$ & $1$ & $2$ & $3$ & $4$ & $5$ & $6$ & $7$ & $8$ & $9$ & $10$ \hline
$s_n$ & $0$ & $1$ & $3$ & $6$ & $10$ & $15$ & $21$ & $28$ & $36$ & $45$ & $55$
\end{array}
\]
Instead of having to perform the summation for each $s_n$, a formula for the sum of the first $n$ integers can be derived.
\begin{thm*}
  $$
    \sum_{k=0}^n k = \frac{n(n+1)}{2}
  $$
\begin{proof}
  Let $s_n=\displaystyle \sum_{k=0}^n k$. Proceed by writing out this sum, then writing out the reversed sum, and then adding the two

\[
  \begin{array}{ccccccccccccccc}
    \setlength{\arraycolsep}{0.01cm}
    $s_n$&$=$&$0$&$+$&$1$&$+$&$2$&$+$&$\cdots$&$+$&$(n-2)$&$+$&$(n-1)$&$+$&$n$
    $s_n$&$=$&$n$&$+$&$(n-1)$&$+$&$(n-2)$&$+$&$\cdots$&$+$&$2$&$+$&$1$&$+$&$0$\hline
    $2s_n$&$=$&$n$&$+$&$n$&$+$&$n$&$+$&$\cdots$&$+$&$n$&$+$&$n$&$+$&$n$
  \end{array}
\]


  There are $n+1$ terms in the sum, therefore
  $$
    2s_n = (n+1)n, \qquad \Rightarrow s_n=\frac{n(n+1)}{2}, \qquad \text{and so } \sum_{k=0}^n k=\frac{n(n+1)}{2}
  $$
\end{proof}
\end{thm*}

* \textbf{Other Series Theorems}
If $a_n$ and $b_n$ are sequences, and $c$ is a constant then,
\[\sum_{k=0}^{n} \left(a_n+b_n\right) = \sum_{k=0}^{n} a_n + \sum_{k=0}^{n}b_n \]
\[\sum_{k=0}^{n} c a_n = c \sum_{k=0}^{n} a_n \]
\[\sum_{k=0}^{n} c = (n+1) c\]


### Arithmetic Series 

And \emph{arithmetic sequence} $a_n$ is a sequences whose terms increase by a constant difference $d$ at each step. And a ***arithmetic series*** $s_n$ is the sum of an arithmetic sequence. Formally
$$
  a_n=a_0+nd, \qquad s_n=\sum_{k=0}^n \left( a_0 + nd \right)
$$
#### Example:

Let $a_n=10+3n$.
\[
\begin{array}{c|c|c|c|c|c|c|c|c}
$n$ & $0$ & $1$ & $2$ & $3$ & $4$ & $5$ & $6$ & $7$   \hline
$a_n$ & $10$ & $13$ & $16$ & $19$ & $22$ & $25$ & $28$ & $31$  \hline
$s_n$ & $10$ & $23$ & $39$ & $58$ & $80$ & $105$ & $133$ & $164$
\end{array}
\]
Instead of having to sum up every term in an arithmetic series, a formula for the $n^{th}$ term in the series can be derived.
\begin{thm*}
  For an arithmetic series
  $$
    s_n = (n+1)\left(a_0 + \frac{n}{2} d\right)
  $$
\begin{proof}
This can be proved by using the theorems on the previous page, in particular using the formula for the sum of the first $n$ integers.
  \begin{align*}
    s_n=\sum_{k=0}^n a_k = \sum_{k=0}^n a_0+kd &= \sum_{k=0}^n a_0+\sum_{k=0}^n kd
    &= (n+1)a_0+d\sum_{k=0}^n k
    &= (n+1)a_0+d\frac{n(n+1)}{2}= \frac{(n+1)}{2} \left( 2a_0+nd\right)
  \end{align*}
\end{proof}
\end{thm*}

* \textbf{Example:} For $a_n=10+3n$, the formula gives
$$
  s_7=(7+1) \left( 10+\dfrac{7}{2} \cdot 3 \right) = 8 \left(  \dfrac{41}{2} \right) = 164
$$
Which matches what was calculated for $s_7$ in the table above. Using the formula, terms even further out can now be calculated without direct summation. For example
\begin{align*}
  s_{100}&=(100+1) \left( 10+\dfrac{100}{2} \cdot 3 \right) = 101 \left(  \dfrac{320}{2} \right) = 16160
  s_{1000}&= 1001 \left( 10+  \dfrac{1000}{2} \cdot 3 \right) =  1511510
\end{align*}


Properties of Sequences {data-navmenu="Section 5"}
==================================

Column {.tabset}
-----------------------------

### Properties of Sequences

#### Boundedness
A sequence is said to be \emph{bounded} if there exists some finite number $M$ such that $|a_n|<M$ for every $n$. A sequence for which no such $M$ exists is said to be \emph{unbounded}.

#### Strictly Positive/Negative
A sequence is \emph{strictly positive} if $a_n > 0$ for all $n$.
A sequence is \emph{strictly negative} if $a_n < 0$ for all $n$.

#### Equivalence
Two sequences $a_n$ and $b_n$ are \emph{equivalent} if $a_n = b_n$ for all $n$.
\textbf{Increasing/Decreasing}
A sequence is \emph{increasing} if $a_{n+1} > a_n$ for all $n$
A sequence is \emph{decreasing} if $a_{n+1} < a_n$ for all $n$

For strictly positive sequences, these conditions mean respectively that $\frac{a_{n+1}}{a_n} > 1$ and $\frac{a_{n+1}}{a_n} < 1$. 
Therefore, to test whether a sequence is increasing or decreasing, the ratio $\frac{a_{n+1}}{a_n}$ must be evaluated.

####  Example:
To test whether the sequence $a_n=n$ is increasing or decreasing.
$$
  a_n=n,\quad a_{n+1}=n+1,\quad \Rightarrow \frac{a_{n+1}}{a_n}=\frac{n+1}{n} > 1 
$$
as $n+1 >n$. Therefore the sequence $a_n=n$ is increasing.

####  Example:

To test whether the sequence $a_n=\frac{n+2}{n+1}$ is increasing or decreasing.

\begin{align*}
  &a_n=\frac{n+2}{n+1},\quad a_{n+1}=\frac{n+3}{n+2},
  &\Rightarrow \frac{a_{n+1}}{a_n}=\frac{\frac{n+3}{n+2}}{\frac{n+2}{n+1}}= \frac{n+3}{n+2}\cdot \frac{n+1}{n+2} = \frac{n^2+4n+3}{n^2+4n+4} = \frac{n^2+4n+3}{\left(n^2+4n+3\right)+1}=\frac{x}{x+1}<1 
\end{align*}
where $x=n^2+4n+2$. Therefore $\frac{a_{n+1}}{a_n}<1$ and so the sequence is decreasing.
